failure characterization

theories/Testing_Pre_orders/Must/Alternative_Preorder/Failure_Set/DefinitionFMS.v
@@ -29,32 +29,34 @@ From Stdlib.Program Require Import Equality.
 From stdpp Require Import finite gmap decidable.
 
 From TestingTheory Require Import ActTau gLts Bisimulation Lts_OBA Subset_Act WeakTransitions Testing_Predicate
-    StateTransitionSystems InteractionBetweenLts Convergence Termination FiniteImageLTS.
+    StateTransitionSystems InteractionBetweenLts Convergence Termination FiniteImageLTS DefinitionAS.
 
-Section failure.
+Definition Failure `{
+  gLtsP : @gLts P A H, CC : Countable PreAct, @FinitaryAbsAction P T FinA PreAct A H Φ 𝝳 _ gLtsEqT _ _ }
+  (p : P) (s : trace A) (G : gset PreAct) :=
+  p ⇓ s -> exists p', p ⟹[s] p' /\ forall β μ, ( 𝝳 ∘ Φ ) β ∈ G -> dual μ β -> blocking β
+  -> ¬ exists p0, p' ⟹{μ} p0.
 
-  Definition Failure `{FiniteImagegLts P A}
-    (p : P) (s : trace A) (G : gset A) :=
-    p ⇓ s -> exists p', p ⟹[s] p' /\ forall μ, μ ∈ G -> ¬ exists p0, p' ⟹{μ} p0.
-
-  Definition fail_pre_ms_cond1 `{gLts P A, gLts Q A} 
+Definition fail_pre_ms_cond1 `{gLts P A, gLts Q A} 
   (p : P) (q : Q) := forall s, p ⇓ s -> q ⇓ s.
 
-  Definition fail_pre_ms_cond2 `{@FiniteImagegLts P A H gLtsP, @FiniteImagegLts Q A H gLtsQ} 
-    (p : P) (q : Q) :=
-    forall s G, Failure q s G -> Failure p s G.
+Notation "p ₁⋖ꜰᴀɪʟ q" := (fail_pre_ms_cond1 p q) (at level 70).
 
-  Definition fail_pre_ms `{@FiniteImagegLts P A H gLtsP, @FiniteImagegLts Q A H gLtsQ} 
-    (p : P) (q : Q) :=
-    fail_pre_ms_cond1 p q /\ fail_pre_ms_cond2 p q.
+Definition fail_pre_ms_cond2 `{ CC : Countable PreAct,
+  gLtsP : @gLts P A H, @FinitaryAbsAction P T FinA PreAct A H Φ 𝝳 _ gLtsEqT _ _ ,
+  gLtsQ : @gLts Q A H, @FinitaryAbsAction Q T FinA PreAct A H Φ 𝝳 _ gLtsEqT _ _ }
+  (p : P) (q : Q) :=
+  forall s G, Failure q s G -> Failure p s G.
 
-End failure.
+Notation "p ₂⋖ꜰᴀɪʟ q" := (fail_pre_ms_cond1 p q) (at level 70).
+
+Definition fail_pre_ms `{ CC : Countable PreAct,
+  gLtsP : @gLts P A H, @FinitaryAbsAction P T FinA PreAct A H Φ 𝝳 _ gLtsEqT _ _ ,
+  gLtsQ : @gLts Q A H, @FinitaryAbsAction Q T FinA PreAct A H Φ 𝝳 _ gLtsEqT _ _ }
+  (p : P) (q : Q) :=
+  fail_pre_ms_cond1 p q /\ fail_pre_ms_cond2 p q.
 
 Global Hint Unfold fail_pre_ms:mdb. 
 
-Notation "p ⋖₁ q" := (fail_pre_ms_cond1 p q) (at level 70).
-
-Notation "p ⋖₂ q" := (fail_pre_ms_cond1 p q) (at level 70).
-
-Notation "p ⋖ q" := (fail_pre_ms p q) (at level 70).
+Notation "p ⋖ꜰᴀɪʟ q" := (fail_pre_ms p q) (at level 70).
 
