theories/Testing_Pre_orders/Must/Alternative_Preorder/Failure_Set/EquivalenceFMS.v
@@ -28,106 +28,173 @@ From Stdlib.Program Require Import Equality.
 
 From stdpp Require Import base decidable gmap finite.
 
-From TestingTheory Require Import gLts Bisimulation Lts_OBA Lts_FW Lts_OBA_FB StateTransitionSystems Termination
-    Must Bar Completeness Soundness Lift Subset_Act FiniteImageLTS WeakTransitions Convergence
-    InteractionBetweenLts MultisetLTSConstruction ForwarderConstruction  ParallelLTSConstruction ActTau
-    Testing_Predicate DefinitionAS DefinitionMS DefinitionFMS EquivalenceMS.
+From TestingTheory Require Import ActTau gLts Bisimulation Lts_OBA Subset_Act WeakTransitions Testing_Predicate
+    StateTransitionSystems InteractionBetweenLts Convergence Termination FiniteImageLTS
+    DefinitionAS DefinitionFMS DefinitionMS EquivalenceMS.
 
-Section failure_must_set.
 
-  Context `{P : Type}.
-  Context `{Q : Type}.
-  Context `{A : Type}.
-  Context `{H : !ExtAction A}.
-
-  Context `{@gLtsObaFB P A H gLtsEqP gLtsObaP, !FiniteImagegLts P A}.
-  Context `{@gLtsObaFB Q A H gLtsEqQ gLtsObaQ, !FiniteImagegLts Q A}.
-
-  Context `{!Prop_of_Inter P (mb A) A fw_inter}.
-  Context `{!Prop_of_Inter Q (mb A) A fw_inter}.
-
-  Lemma equivalence_must_set_nfailure
-    (p : P) (s : trace A) h1 (G : gset A) :
-    MUST__s (AFTER (p, ∅) s h1) G
-      <-> ¬ Failure (p, ∅) s G.
-  Proof.
-    split.
-    - intros hm (e & hw & hf). eassumption.
-      edestruct (hm e) as (μ & p' & mem' & hw'). eapply wt_set_spec2. eauto. eapply wt_nil.
-      edestruct (hf μ mem'). eauto.
-    - intros hnf.
-      assert (∀ p0 : P * mb A, p0 ∈ AFTER (p ▷ ∅) s h1 → p0 ⇓ []).
-      intros p0 mem0. eapply cnv_nil, cnv_wt_s_terminate; eauto.
-      eapply (wt_set_spec1 _ _ _ _ mem0).
-      destruct (either_MUST__s (AFTER (p, ∅) s h1) G) as [Hyp | Hyp]; eauto.
-      + eapply nMusts_ex in Hyp as (p0 & mem & hnm).
-        exfalso. eapply hnf.
+Lemma equivalence_must_set_nfailure `{
+  gLtsP : @gLts P A H, !FiniteImagegLts P A, CC : Countable PreAct,
+  @FinitaryAbsAction P T FinA PreAct A H Φ 𝝳 _ gLtsEqT _ _}
+  (p : P) (s : trace A) h1 (G : gset PreAct) : MUST__s (AFTER p s h1) G <->  ¬ Failure p s G.
+Proof.
+  split.
+  - intros hm (e & hw & hf). eassumption.
+    edestruct (hm e) as (β & μ & p' & mem' & hw' & duo & b). eapply wt_set_spec2. eauto. eapply wt_nil.
+    edestruct (hf β μ mem' duo b). eauto.
+  - intros hnf.
+    assert (∀ p0 : P, p0 ∈ AFTER p s h1 → p0 ⇓ []).
+    { intros p0 mem0. eapply cnv_nil, cnv_wt_s_terminate; eauto.
+      eapply (wt_set_spec1 _ _ _ _ mem0). }
+    destruct (either_MUST__s (AFTER p s h1) G) as [Hyp | Hyp]; eauto.
+    + eapply nMusts_ex in Hyp as (p0 & mem & hnm).
+      * exfalso. eapply hnf.
         eapply nMust_ex in hnm as (p1 & hw1 & hnp).
         exists p1. split.
         eapply wt_push_nil_right.
         eapply (wt_set_spec1 _ _ _ _ mem). eassumption.
-        intros μ mem0 (p' & hw'). eapply hnp. eassumption.
-        eassumption.
+        intros β μ mem0 duo b (p' & hw'). eapply hnp. eassumption.
+        eassumption. eassumption. eassumption.
         eapply cnv_nil, cnv_wt_s_terminate; eauto.
-        eapply (wt_set_spec1 _ _ _ _ mem). eauto.
-  Qed.
+        eapply (wt_set_spec1 _ _ _ _ mem).
+      * eauto.
+Qed.
 
-  Lemma equivalence_nmust_set_failure
-    (p : P) (s : trace A) h1 (G : gset A) :
-    ¬ MUST__s (AFTER (p ▷ ∅) s h1) G
-      <-> Failure (p ▷ ∅) s G.
-  Proof.
-    split.
-    - intro hm.
-      eapply nMusts_ex in hm as (p0 & mem & hnm).
-      eapply nMust_ex in hnm as (p1 & hw1 & hnp).
-      exists p1. split.
-      eapply wt_push_nil_right.
-      eapply (wt_set_spec1 _ _ _ _ mem). eassumption.
-      intros μ mem0 (p' & hw'). eapply hnp. eassumption.
-      eassumption.
-      eapply cnv_nil, cnv_wt_s_terminate; eauto.
-      eapply (wt_set_spec1 _ _ _ _ mem).
-      intros p0 mem0. eapply cnv_nil, cnv_wt_s_terminate; eauto.
-      eapply (wt_set_spec1 _ _ _ _ mem0).
-    - intros (e & hmem & hf) hm. eassumption.
-      unfold MUST__s in hm.
-      edestruct (hm e) as (μ & p1 & mem1 & hw1).
-      eapply (wt_set_spec2 _ _ _ _ hmem). eapply wt_nil.
-      eapply (hf μ mem1). eauto.
-  Qed.
+Lemma equivalence_nmust_set_failure `{
+  gLtsP : @gLts P A H, !FiniteImagegLts P A, CC : Countable PreAct,
+  @FinitaryAbsAction P T FinA PreAct A H Φ 𝝳 _ gLtsEqT _ _}
+  (p : P) (s : trace A) h1 (G : gset PreAct) :
+  ¬ MUST__s (AFTER p s h1) G
+    <-> Failure p s G.
+Proof.
+  split.
+  - intro hm.
+    eapply nMusts_ex in hm as (p0 & mem & hnm).
+    eapply nMust_ex in hnm as (p1 & hw1 & hnp).
+    exists p1. split.
+    eapply wt_push_nil_right.
+    eapply (wt_set_spec1 _ _ _ _ mem). eassumption.
+    intros β μ mem0 duo b (p' & hw'). eapply hnp. eassumption.
+    eassumption. eassumption. eassumption.
+    eapply cnv_nil, cnv_wt_s_terminate; eauto.
+    eapply (wt_set_spec1 _ _ _ _ mem).
+    intros p0 mem0. eapply cnv_nil, cnv_wt_s_terminate; eauto.
+    eapply (wt_set_spec1 _ _ _ _ mem0).
+  - intros (e & hmem & hf) hm. eassumption.
+    unfold MUST__s in hm.
+    edestruct (hm e) as (β & μ & p1 & mem1 & hw1 & duo & b).
+    eapply (wt_set_spec2 _ _ _ _ hmem). eapply wt_nil.
+    eapply (hf β μ mem1 duo b). eauto.
+Qed.
 
-End failure_must_set.
+Theorem equivalence_failure_set_must_set `{ CC : Countable PreAct,
+  gLtsP : @gLts P A H, !FiniteImagegLts P A,
+  @FinitaryAbsAction P T FinA PreAct A H Φ 𝝳 _ gLtsEqT _ _,
+  gLtsQ : @gLts Q A H, !FiniteImagegLts Q A,
+  @FinitaryAbsAction Q T FinA PreAct A H Φ 𝝳 _ gLtsEqT _ _
+  }
+  (p : P) (q : Q) : p ≾ₘᵤₛₜ q <-> p ⋖ꜰᴀɪʟ q.
+Proof.
+  split.
+  - intros (hpre1 & hpre2). split.
+    + exact hpre1.
+    + intros s G hf hcnv.
+      eapply (equivalence_nmust_set_failure p s hcnv).
+      intros hm. eapply (hpre2 s hcnv (hpre1 s hcnv)) in hm.
+      eapply (equivalence_must_set_nfailure q s (hpre1 s hcnv) G) in hm. contradiction. eassumption.
+  - intros (hpre1 & hpre2). split. 
+    + exact hpre1. 
+    + intros s h1 h2 G hm%equivalence_must_set_nfailure.
+      eapply (equivalence_must_set_nfailure q).
+      intros hf%hpre2. contradiction.
+Qed.
 
-Section failure_must_set_pre.
+
+From stdpp Require Import base decidable gmap finite.
+From Stdlib Require Import ssreflect.
+From Stdlib.Program Require Import Equality.
+From TestingTheory Require Import gLts Bisimulation Lts_OBA Lts_FW Lts_OBA_FB StateTransitionSystems Termination
+    Must Bar Completeness Soundness Lift Subset_Act FiniteImageLTS WeakTransitions Convergence
+    InteractionBetweenLts MultisetLTSConstruction ForwarderConstruction ParallelLTSConstruction ActTau
+    Testing_Predicate DefinitionAS MustE Lts_Finite_Output_Chain Equivalence Soundness Completeness.
+
+Section failure_set_preorder.
+  Context `{outcome : T -> Prop}.
+  Context `{outcome_dec : forall t, Decision (outcome t)}.
   Context `{P : Type}.
   Context `{Q : Type}.
-  Context `{A : Type}.
   Context `{H : !ExtAction A}.
 
-  Context `{@gLtsObaFB P A H gLtsEqP gLtsObaP, !FiniteImagegLts P A}.
-  Context `{@gLtsObaFB Q A H gLtsEqQ gLtsObaQ, !FiniteImagegLts Q A}.
+  Context `{@gLtsOba P A H gLtsEqP, !FiniteImagegLts P A}.
+  Context `{@gLtsOba Q A H gLtsEqQ, !FiniteImagegLts Q A}.
+  Context `{@gLtsOba T A H gLtsEqT, !FiniteImagegLts T A, !Testing_Predicate outcome _}.
 
-  Context `{!Prop_of_Inter P (mb A) A fw_inter}.
-  Context `{!Prop_of_Inter Q (mb A) A fw_inter}.
+  Context `{!Prop_of_Inter P T A dual}.
+  Context `{!Prop_of_Inter Q T A dual}.
 
-  Theorem equivalence_pre_failure_must_set
+  Context `{!Prop_of_Inter P (MO A) A fw_inter}.
+  Context `{!Prop_of_Inter (P * MO A) T A dual}.
+  Context `{!Prop_of_Inter Q (MO A) A fw_inter}.
+  Context `{!Prop_of_Inter (Q * MO A) T A dual}.
 
-  (p : P) (q : Q) : (p ▷ ∅) ≾ₘᵤₛₜ (q ▷ ∅) <-> (p ▷ ∅) ⋖ (q ▷ ∅).
+
+  Context `{CC : Countable PreAct}.
+  Context `{@FinitaryAbsAction P T FinA PreAct A H Φ 𝝳 _ _ _ _ }.
+  Context `{@FinitaryAbsAction Q T FinA PreAct A H Φ 𝝳 _ _ _ _ }.
+
+  Context `{tc_spec : @test_convergence_spec T _ _ _ outcome _ t_conv}.
+  Context `{ta_spec : @test_co_acceptance_set_spec PreAct _ _ T _ _ _ outcome Testing_Predicate0 ta (fun x => 𝝳 (Φ x))}.
+
+  (** * Main equivalence theorems *)
+
+  Section FWⁿ.
+
+  Context `{!gLtsObaFW P A}.
+  Context `{!gLtsObaFW Q A}.
+  Context `{!gLtsObaFB T A}.
+
+  (** ** The must-set characterisation on FW is equivalent to the extensional must preorder *)
+  Corollary equivalence_fw_failure_set_and_must_e (p : P) (q : Q) :
+    p ⋖ꜰᴀɪʟ q <-> pre_extensional outcome p q.
   Proof.
-    split.
-    - intros (hpre1 & hpre2). split.
-      + exact hpre1.
-      + intros s G hf hcnv.
-        eapply (equivalence_nmust_set_failure p s hcnv).
-        intros hm. eapply (hpre2 s hcnv (hpre1 s hcnv)) in hm.
-        eapply (equivalence_must_set_nfailure q s (hpre1 s hcnv) G) in hm. contradiction. eassumption.
-    - intros (hpre1 & hpre2). split. 
-      + exact hpre1. 
-      + intros s h1 h2 G hm%equivalence_must_set_nfailure.
-        eapply (equivalence_must_set_nfailure q).
-        intros hf%hpre2. contradiction.
+    erewrite<- equivalence_failure_set_must_set.
+    rewrite equivalence_fw_must_set_and_must_e;eauto.
   Qed.
 
-End failure_must_set_pre.
+  (** ** The must-set characterisation on FW is equivalent to the inductive must preorder *)
+  Corollary equivalence_fw_failure_set_and_must_i (p : P) (q : Q) :
+     p ⋖ꜰᴀɪʟ q <-> p ⊑ₘᵤₛₜᵢ q .
+  Proof.
+    erewrite<- equivalence_failure_set_must_set.
+    rewrite equivalence_fw_must_set_and_must_i;eauto.
+  Qed.
+
+  End FWⁿ.
+  (** ---- *)
+  Section Lⁿ.
+
+  Context `{!gLtsObaFB P A, !FiniteOutputChain_LtsOba P}.
+  Context `{!gLtsObaFB Q A, !FiniteOutputChain_LtsOba Q}.
+  Context `{!gLtsObaFB T A, !FiniteOutputChain_LtsOba T}.
+
+  (** ** The must-set characterisation on toFW is equivalent to the inductive must preorder *)
+  Corollary equivalence_failure_set_and_must_i (p : P) (q : Q) :
+    p ⊑ₘᵤₛₜᵢ q <-> (p, ∅) ⋖ꜰᴀɪʟ (q, ∅).
+  Proof.
+    erewrite<- equivalence_failure_set_must_set.
+    rewrite equivalence_must_set_and_must_i; eauto.
+  Qed.
+
+  (** ---- *)
+
+  (** ** The inductive characterisation on toFW is equivalent to the extensional must preorder *)
+  Corollary equivalence_failure_set_and_must_e (p : P) (q : Q) :
+    pre_extensional outcome p q <-> (p, ∅) ⋖ꜰᴀɪʟ (q, ∅).
+  Proof.
+    rewrite pre_extensional_eq. apply equivalence_failure_set_and_must_i.
+  Qed.
+
+  End Lⁿ.
+
+End failure_set_preorder.
 
